TestTheories/Sorting.thy
@@ -4,23 +4,29 @@ imports Main
         Listing
 begin
 
-fun sorted :: "Nat List \<Rightarrow> bool" where
+fun sorted :: "nat List \<Rightarrow> bool" where
   "sorted Nil                   = True"
 | "sorted (Cons _ Nil)          = True"
-| "sorted (Cons r (Cons t ts))  = (leq r t \<and> sorted (Cons t ts))"
+| "sorted (Cons r (Cons t ts))  = ( r \<le> t \<and> sorted (Cons t ts))"
 
-fun insert :: "Nat \<Rightarrow> Nat List \<Rightarrow> Nat List" where
+fun insert :: "nat \<Rightarrow> nat List \<Rightarrow> nat List" where
   "insert r Nil         = Cons r Nil"
-| "insert r (Cons t ts) = (if leq r t then Cons r (Cons t ts) else (Cons t (insert r ts)))"
+| "insert r (Cons t ts) = (if r \<le> t then Cons r (Cons t ts) else (Cons t (insert r ts)))"
 
 
-fun isort :: "Nat List \<Rightarrow> Nat List" where
+fun isort :: "nat List \<Rightarrow> nat List" where
   "isort Nil = Nil"
 | "isort (Cons t ts) = insert t (isort ts)"
 
-fun qsort :: "Nat list \<Rightarrow> Nat list" where
+fun qsort :: "nat list \<Rightarrow> nat list" where
   "qsort [] = []"
-| "qsort (t # ts) = [r . r <- ts, leq r t] @ (t # [r . r <- ts, \<not> (leq r t)])"
+| "qsort (t # ts) = [r . r <- ts, r \<le> t] @ (t # [r . r <- ts, \<not> (r \<le> t)])"
+
+fun sorted' :: "nat list \<Rightarrow> bool" where
+  "sorted' []                   = True"
+| "sorted' [x]         = True"
+| "sorted' (r # (t # ts))  = (r \<le> t \<and>  sorted' (t # ts))"
+
 (*
 fun merge :: "Nat list \<Rightarrow> Nat list \<Rightarrow> Nat list" where
   "merge [] ts = ts"
