TestTheories/Turtle.thy
@@ -1,0 +1,139 @@
+theory Turtle
+imports Main
+
+begin
+
+type_synonym angle = int
+type_synonym point = "int * int"
+type_synonym distance = int
+
+record turtle =     facing :: angle
+                    loc :: point
+                    fly :: bool
+
+type_synonym instant = "((turtle * turtle) * string) list"
+type_synonym transiton = "turtle \<Rightarrow> turtle option"
+
+datatype prog = Empty "(prog list)" | Node transiton "(prog list)"
+
+fun endPoint :: "point \<Rightarrow> angle \<Rightarrow> distance \<Rightarrow> point" where
+  "endPoint (x, y) d l = (x + l * d, y + l * d)"
+
+fun moveT :: "distance \<Rightarrow> turtle \<Rightarrow> turtle" where
+  "moveT n t = t \<lparr> loc := endPoint (loc t) (facing t) n \<rparr>"
+
+fun rotateT :: "angle \<Rightarrow> turtle \<Rightarrow> turtle" where
+  "rotateT d t = t \<lparr> facing := (facing t + d) mod 6 \<rparr>"
+
+definition initTurtle :: "turtle" where
+  "initTurtle = \<lparr> facing = 0, loc = (0, 0), fly = False\<rparr>"
+
+definition empty :: "prog" where
+ "empty = Empty []"
+
+fun K :: "'b \<Rightarrow> 'a \<Rightarrow> 'b" where
+  "K b x = b"
+
+definition die :: "prog" where
+  "die = Node (K None) []"
+
+fun transit :: "(turtle \<Rightarrow> turtle) \<Rightarrow> prog" where
+  "transit f = Node (Some o f) []"
+
+definition idle :: "prog" where
+  "idle = transit id"
+
+definition penup :: "prog" where
+  "penup = transit (\<lambda> t. t \<lparr>fly := True\<rparr>)"
+
+definition pendown :: "prog" where
+  "pendown = transit (\<lambda> t. t \<lparr>fly := False\<rparr>)"
+
+fun forward :: "distance \<Rightarrow> prog" where
+  "forward n = transit (moveT n)"
+
+fun backward :: "distance \<Rightarrow> prog" where
+  "backward n = transit (moveT (- n))"
+
+fun right :: "angle \<Rightarrow> prog" where
+  "right d = transit (rotateT (- d))"
+
+fun left :: "angle \<Rightarrow> prog" where
+  "left d = transit (rotateT d)"
+
+fun getCh :: "prog \<Rightarrow> prog list" where
+  "getCh (Empty  cs) = cs"
+| "getCh (Node _ cs) = cs"
+
+fun getOp :: "prog \<Rightarrow> prog list \<Rightarrow> prog" where
+  "getOp (Empty  _) = Empty"
+| "getOp (Node t _) = Node t"
+
+fun inject :: "int \<Rightarrow> prog \<Rightarrow> (int \<Rightarrow> prog \<Rightarrow> bool) \<Rightarrow> (prog \<Rightarrow> prog \<Rightarrow> prog) \<Rightarrow> prog \<Rightarrow> prog" where
+  "inject n new fcond gtrans p =
+    (if fcond n p then gtrans new p
+                  else getOp p (map (inject ((\<lambda>p . case p of Empty _ \<Rightarrow> n
+                                                           | Node _ _ \<Rightarrow> n + 1) p) new fcond gtrans) (getCh p)))"
+
+fun append :: "int \<Rightarrow> prog \<Rightarrow> (int \<Rightarrow> prog \<Rightarrow> bool) \<Rightarrow> prog \<Rightarrow> prog" where
+  "append n new f = inject n new f (\<lambda>r p. getOp p [r])"
+
+fun isLeaf :: "prog \<Rightarrow> bool" where
+  "isLeaf p = null (getCh p)"
+
+fun isLastAction :: "prog \<Rightarrow> bool" where
+  "isLastAction = isLeaf"
+
+fun hasEmptyAction :: "prog \<Rightarrow> bool" where
+  "hasEmptyAction (Empty _) = True"
+| "hasEmptyAction _         = False"
+
+fun isEmpty :: "prog \<Rightarrow> bool" where
+  "isEmpty (Empty []) = True"
+| "isEmpty (Empty cs) = list_all isEmpty cs"
+| "isEmpty _          = False"
+
+fun seq :: "program \<Rightarrow> program \<Rightarrow> program" where  (infixr " >*>" 65)
+  "seq p q = append 0 q (\<lambda>x. isLeaf x) p"
+
+-- | Parallel combinator: execution of two programs in parallel
+(<|>) :: Program -> Program -> Program
+p <|> q = Empty [p, q]
+
+-- | Setting a lifespan
+lifespan :: Int -> Program -> Program
+lifespan n = replace 0 die (\i _ -> i == n)
+
+-- | Limiting operations in time
+limited :: Int -> Program -> Program
+limited n = replace 0 (Empty []) (\i _ -> i == n)
+
+-- | Creates a program repeating the program parameter a finite number of times
+times :: Int -> Program -> Program
+times n p | n <= 0    = Empty []
+          | otherwise = p >*> times (n-1) p 
+
+-- | Creates a program repeating the program parameter infinitely
+forever :: Program -> Program
+forever p = p >*> forever p
+
+
+
+-- | Returns the first action in a program. Such an action is a function
+-- 
+--   >  [Program] -> Program
+--
+-- which sequences a list of programs (to occur in parallel) after the first
+-- operation in the program parameter.
+firstAction :: Program -> [Program] -> Program
+firstAction = getOp
+
+-- | Returns all programs occurring in paralell after the first operation
+-- in the program
+restActions :: Program -> [Program]
+restActions = getCh
+
+
+
+end
+
